Splinter/AllocationsLayer/AllocationJournal.i.dfy
@@ -54,7 +54,7 @@ module AllocationJournal {
 
   datatype TransitionLabel =
       ReadForRecoveryLabel(messages: MsgHistory)
-    | FreezeForCommitLabel(frozenJournal: JournalImage)
+    | FreezeForCommitLabel(frozenJournal: JournalImage, unobserved: set<AU>)
     | QueryEndLsnLabel(endLsn: LSN)
     | PutLabel(messages: MsgHistory)
     | DiscardOldLabel(startLsn: LSN, requireEnd: LSN, deallocs: set<AU>)
@@ -69,7 +69,7 @@ module AllocationJournal {
     function I(): LikesJournal.TransitionLabel {
       match this {
         case ReadForRecoveryLabel(messages) => LikesJournal.ReadForRecoveryLabel(messages)
-        case FreezeForCommitLabel(frozenJournal) => LikesJournal.FreezeForCommitLabel(frozenJournal.tj)
+        case FreezeForCommitLabel(frozenJournal, _) => LikesJournal.FreezeForCommitLabel(frozenJournal.tj)
         case QueryEndLsnLabel(endLsn) => LikesJournal.QueryEndLsnLabel(endLsn)
         case PutLabel(messages) => LikesJournal.PutLabel(messages)
         case DiscardOldLabel(startLsn, requireEnd, _) => LikesJournal.DiscardOldLabel(startLsn, requireEnd)
@@ -95,11 +95,6 @@ module AllocationJournal {
       && miniAllocator.WF()
     }
 
-    function UnobservedAUs() : set<AU>
-    {
-      miniAllocator.NotObservedAUs()
-    }
-
     function AccessibleAUs() : set<AU>
     {
       lsnAUIndex.Values + miniAllocator.allocs.Keys
@@ -117,6 +112,14 @@ module AllocationJournal {
     )
   }
 
+  // should ==  G.ToAUs(frozenjournal.tj.diskview.keys)
+  function frozenAUs(frozenJournal: JournalImage, lsnAUIndex: map<LSN, AU>) : (out: set<AU>)
+    requires frozenJournal.WF()
+  {
+    var frozenLSNs := set lsn | frozenJournal.tj.SeqStart() <= lsn < frozenJournal.tj.SeqEnd();
+    MapRestrict(lsnAUIndex, frozenLSNs).Values
+  }
+
   predicate FreezeForCommit(v: Variables, v': Variables, lbl: TransitionLabel, step: Step)
   {
     && v.WF()
@@ -124,6 +127,8 @@ module AllocationJournal {
     && step.FreezeForCommitStep?
 
     && LikesJournal.FreezeForCommit(v.journal, v'.journal, lbl.I(), step.depth)
+    && lbl.unobserved == v.AccessibleAUs() - frozenAUs(lbl.frozenJournal, v.lsnAUIndex)
+
     && v' == v.(
       journal := v'.journal
     )
